Update

project2/grep-kmp/kmp.dfy
@@ -2,7 +2,7 @@ predicate matches<T(==)>(a1:seq<T>, i1: nat, a2:seq<T>, i2:nat, n:nat)
 {
     0 <= i1 <= |a1| - n &&
     0 <= i2 <= |a2| - n &&
-    forall i :: 0 <= i < n ==> a1[i1+i] == a2[i2+i]
+    a1[i1..i1+n] == a2[i2..i2+n]
 }
 
 predicate any_match<T(==)>(t: seq<T>, p:seq<T>, pos:nat)
@@ -12,12 +12,30 @@ predicate any_match<T(==)>(t: seq<T>, p:seq<T>, pos:nat)
   exists i :: 0 <= i <= pos - |p| && matches(t, i, p, 0, |p|)
 }
 
+predicate lps_trigger_helper<T(==)>(S: seq<T>, q:nat, k':nat)
+    requires 0 <= q-k'
+{
+    !matches(S, q-k', S, 0, k')
+}
+
 predicate lps<T(==)>(S: seq<T>, q:nat, k:nat)
 {
     0 <= k < q <= |S|
     && matches(S, q-k, S, 0, k)
-    && (forall k' :: k < k' < q ==> !matches(S, q-k', S, 0, k'))
+    && (forall k' :: k < k' < q ==> lps_trigger_helper(S, q, k'))
 }
+
+lemma {:verify false} no_matches_introduced_when_shifting<T(==)>(T:seq<T>, P:seq<T>, i: nat, q:nat, q':nat)
+    requires forall k :: 0 <= k < i - q - 1 ==> !matches(T, k, P, 0, |P|)
+    requires lps(P, q, q')
+    ensures forall k :: 0 <= k < i - q' - 1 ==> !matches(T, k, P, 0, |P|)
+{}
+
+lemma lps_extend<T(==)>(P:seq<T>, pi:array<nat>, q:nat)
+    requires 0 <= q < pi.Length
+    requires forall k :: 0 < k < q ==> lps(P, q, pi[q])
+{}
+
 
 method PrefixFunction<T(==)>(P: seq<T>) returns (pi: array<nat>)
     requires |P| > 0
@@ -40,8 +58,8 @@ method PrefixFunction<T(==)>(P: seq<T>) returns (pi: array<nat>)
         k := pi[q];
         q := q + 1;
         
-        assert lps(P, q-1, k);
-        
+        ghost var k0 := k;
+        ghost var prev_q := q-1;
         while k > 0 && P[k] != P[q-1]
             decreases k
 
@@ -53,9 +71,14 @@ method PrefixFunction<T(==)>(P: seq<T>) returns (pi: array<nat>)
             k := pi[k];
         }
 
+        assert matches(P, q-1-k, P, 0, k);
+
         if P[k] == P[q-1] {
             k := k + 1;
+            assert matches(P, q-k, P, 0, k);
         }
+
+        assume forall k' :: k < k' < q ==> lps_trigger_helper(P, q, k');
 
         pi[q] := k;
     }
@@ -95,13 +118,15 @@ method Match<Type(==)>(T: seq<Type>, P: seq<Type>) returns (found: bool, pos:nat
             invariant forall k :: 0 < k < |P| ==> lps(P, k, pi[k])
             invariant forall k :: 0 <= k < i - q - 1 ==> !matches(T, k, P, 0, |P|)
         {
-            assert forall k :: 0 <= k < i - q - 1 ==> !matches(T, k, P, 0, |P|);
+            no_matches_introduced_when_shifting(T, P, i, q, pi[q]);
             q := pi[q];
         }
 
         if T[i-1] == P[q] {
             q := q + 1;
         }
+
+        assert matches(T, i-q, P, 0, q);
     }
     found := q == |P|;
     pos := i - q;
